default ghost names now set to 1%positive; sWorld.v -> syn_invariants

iris_system/syn_invariants.v
@@ -26,7 +26,7 @@ Global Instance inv_syntax : PF.t := {
 }.
 
 (* Invariant interpretations *)
-Local Definition inv_interp_aux `{α : SRFCons.t, Γ : HRA, !subG Γ Σ, !invGS Σ Γ} n (s : inv_shape) :
+Local Definition inv_interp_aux `{α : SRFCons.t, Γ : HRA, !subG Γ Σ, !invG Σ Γ} n (s : inv_shape) :
     (inv_degree s (SRFSyn.t_prev n) → SRFSyn.t n) → (inv_degree s (SRFSyn.t_prev n) → iProp Σ)
     → iProp Σ :=
   match s with
@@ -35,14 +35,15 @@ Local Definition inv_interp_aux `{α : SRFCons.t, Γ : HRA, !subG Γ Σ, !invGS 
   | _wsat_auth u => λ _ _, wsat_auth u n
   end.
 
-Global Instance inv_interp `{α : SRFCons.t, Γ : HRA, !subG Γ Σ, !invGS Σ Γ} :
+Global Instance inv_interp `{α : SRFCons.t, Γ : HRA, !subG Γ Σ, !invG Σ Γ} :
     @SRFIntpM.t (@domain Σ) α _ :=
   inv_interp_aux.
 
 Section syn_inv.
   Context `{Γ : HRA} `{!subG Γ Σ} `{!CtxST.t τ} `{!SRFIntp.inG SL.syntax α SL.t β}.
-  Context `{!invGS Σ Γ, !SRFIntp.inG _ α inv_interp β}.
-  Local Existing Instances inv_preΣ inv_preΓ invGS_I invGS_E invGS_D.
+  Context `{!invG Σ Γ, !SRFIntp.inG _ α inv_interp β}.
+  Local Existing Instances invG_Σ invG_Γ invG_I invG_E invG_D.
+  (* Local Existing Instances inv_preΣ inv_preΓ invG_I invG_E invG_D. *)
 
   Local Definition syn_ownI u n i (p : SRFSyn.t n) : SRFSyn.t n :=
     ⟨ _ownI u i, λ _, p ⟩.
@@ -52,11 +53,11 @@ Section syn_inv.
     ⟨ _wsat_auth u, λ e, match e with end ⟩.
 
   Local Definition syn_ownE (u : univ_id) n (E : coPset) : SRFSyn.t n :=
-    <own> enabled_name (ownER u E).
+    <own> 1%positive (ownER u E).
   Local Definition syn_ownD (u : univ_id) n (D : gset positive) : SRFSyn.t n :=
-    <own> disabled_name (ownDR u D).
+    <own> 1%positive (ownDR u D).
   Local Definition syn_ownD_auth (u : univ_id) n : SRFSyn.t n :=
-    (∃ D : τ{⇣gset positive}, <own> disabled_name (ownD_authR u D))%SRF.
+    (∃ D : τ{⇣gset positive}, <own> 1%positive (ownD_authR u D))%SRF.
 
   Local Definition syn_inv_satall u n (I : gmap positive (SRFSyn.t n)) : SRFSyn.t n :=
     ([∗ n map] i ↦ p ∈ I, (p ∗ syn_ownD u n {[i]}) ∨ syn_ownE u n {[i]})%SRF.
@@ -85,17 +86,17 @@ Section syn_inv.
   Local Definition syn_fupd_eq : @syn_fupd = @syn_fupd_def := syn_fupd_aux.(seal_eq).
 End syn_inv.
 
-Class sinvGS (Σ : GRA) (Γ : HRA) α β τ := {
+Class sinvG (Σ : GRA) (Γ : HRA) α β τ := {
   #[global] sinv_subG :: subG Γ Σ;
   #[global] sinv_typG :: CtxST.t τ;
   #[global] sinv_SL_intpG :: SRFIntp.inG SL.syntax α SL.t β;
-  #[global] sinv_invGS :: invGS Σ Γ;
+  #[global] sinv_invG :: invG Σ Γ;
   #[global] sinv_inv_intpG :: SRFIntp.inG inv_syntax α inv_interp β;
-  sinv_dom := domain Σ
+  (* sinv_dom := domain Σ *)
 }.
 
 Section reduction.
-  Context `{!sinvGS Σ Γ α β τ}.
+  Context `{!sinvG Σ Γ α β τ}.
   Lemma ownI_auth_red u n I :
     ⟦syn_ownI_auth u n I⟧ = ownI_auth u n I.
   Proof.
@@ -164,7 +165,7 @@ Ltac inv_red :=
     try rewrite ! fupd_red
   ).
 
-Module Adequacy.
+Module inv_instances.
   Instance τ : Typ.t := λ _, ST.t.
 
   Instance typG : CtxST.t τ.
@@ -177,21 +178,21 @@ Module Adequacy.
       | _ => inv_syntax
       end.
 
-  Instance β {Σ : GRA} {Γ : HRA} `{!subG Γ Σ, !invGS Σ Γ} : SRFIntp.t :=
+  Instance β {Σ : GRA} {Γ : HRA} `{!subG Γ Σ, !invG Σ Γ} : SRFIntp.t :=
     λ n,
       match n with
       | 0 => SL.t
       | _ => inv_interp
       end.
 
-  Instance intpG {Σ : GRA} {Γ : HRA} `{!subG Γ Σ, !invGS Σ Γ} :
+  Instance intpG {Σ : GRA} {Γ : HRA} `{!subG Γ Σ, !invG Σ Γ} :
     SRFIntp.inG (@SL.syntax τ Γ) α (@SL.t τ α Γ Σ _) β.
   Proof. econs; instantiate (1:=0); ss. Qed.
 
-  Instance invintpG {Σ : GRA} {Γ : HRA} `{!subG Γ Σ, !invGS Σ Γ} :
+  Instance invintpG {Σ : GRA} {Γ : HRA} `{!subG Γ Σ, !invG Σ Γ} :
     SRFIntp.inG inv_syntax α inv_interp β.
   Proof. econs; instantiate (1:=1); ss. Qed.
 
-  Instance sinvgs {Σ : GRA} {Γ : HRA} `{!subG Γ Σ, !invGS Σ Γ} : sinvGS Σ Γ α β τ.
+  Instance sinvg {Σ : GRA} {Γ : HRA} `{!subG Γ Σ, !invG Σ Γ} : sinvG Σ Γ α β τ.
   Proof. econs; try typeclasses eauto. Qed.
-End Adequacy.
+End inv_instances.
